HoareLogicRefine.v: some minor cleanup
trying to prove the refined read (onestate), but it appears difficult
due to the disconnected pre- and post-conditions, and the abuse of the
ghost variable in Call.

src/HoareLogicRefine.v
@@ -28,17 +28,17 @@ Module Type ONEINT.
 End ONEINT.
 
 Module Oneint : ONEINT.
-  Definition read xp := $((mem*mem):
-    (Call (fun ms : mem*mem => Log.begin_ok xp (fst ms)));;
-    x <- (Call (fun ms : mem*mem => Log.read_ok xp 3 ms));
-    (Call (fun ms : mem*mem => Log.commit_ok xp (fst ms) (snd ms)));;
+  Definition read xp := $(mem:
+    (Call (fun m : mem => Log.begin_ok xp m));;
+    x <- (Call (fun m : mem => Log.read_ok xp 3 (m, m)));
+    (Call (fun m : mem => Log.commit_ok xp m m));;
     (Halt x)
   ).
 
-  Definition write xp v := $((mem*mem):
-    (Call (fun ms : mem*mem => Log.begin_ok xp (fst ms)));;
-    (Call (fun ms : mem*mem => Log.write_ok xp 3 v ms));;
-    (Call (fun ms : mem*mem => Log.commit_ok xp (fst ms) (snd ms)))
+  Definition write xp v := $(mem:
+    (Call (fun m : mem => Log.begin_ok xp m));;
+    (Call (fun m : mem => Log.write_ok xp 3 v (m, upd m 3 v)));;
+    (Call (fun m : mem => Log.commit_ok xp m (upd m 3 v)))
   ).
 
   Definition rep xp (os: onestate) :=
@@ -48,7 +48,7 @@ Module Oneint : ONEINT.
       [lm (DataStart xp + 3) = a]
     end%pred.
 
-  Theorem read_ok : forall xp a (ms:mem*mem),
+  Theorem read_ok : forall xp a (m:mem),
     {{rep xp (One a) /\
       [DataStart xp <= 3 < DataStart xp + DataLen xp]}}
     (read xp)
